Fix to enable to use read permission in kernelInv

Compiler/Correctness.v
@@ -28,9 +28,9 @@ Definition arr2CUDA {ty} : Skel.aTypDenote ty -> list (vals ty) := map sc2CUDA.
 Definition val2sh {ty} := @maptys ty _ _ SLoc.
 Definition val2gl {ty} := @maptys ty _ _ GLoc.
 
-Definition arrInvRes {GA} (aPtrEnv : APtrEnv GA) (aEvalEnv : AEvalEnv GA) : res :=
+Definition arrInvRes {GA} (aPtrEnv : APtrEnv GA) (aEvalEnv : AEvalEnv GA) p : res :=
   fold_hlist GA Star Emp
-    (fun x m => arrays (val2gl (hget aPtrEnv m)) (arr2CUDA (hget aEvalEnv m)) 1).
+    (fun x m => arrays (val2gl (hget aPtrEnv m)) (arr2CUDA (hget aEvalEnv m)) p).
 
 Definition arrInvVar {GA} (aVarEnv : AVarEnv GA) (aPtrEnv : APtrEnv GA) (aEvalEnv : AEvalEnv GA) : list entry :=
   fold_hlist GA (@app entry) nil
@@ -43,14 +43,14 @@ Definition scInv {GS} (sVarEnv : SVarEnv GS) (sEvalEnv : SEvalEnv GS) :=
 
 Definition sexpInv {GS GA}
            (sVarEnv : SVarEnv GS) (sEvalEnv : SEvalEnv GS)
-           (aVarEnv : AVarEnv GA) (aPtrEnv : APtrEnv GA) (aEvalEnv : AEvalEnv GA) R P resEnv :=
-  Assn (arrInvRes aPtrEnv aEvalEnv *** R)
+           (aVarEnv : AVarEnv GA) (aPtrEnv : APtrEnv GA) (aEvalEnv : AEvalEnv GA) R P resEnv p :=
+  Assn (arrInvRes aPtrEnv aEvalEnv p *** R)
        P
        (resEnv ++ scInv sVarEnv sEvalEnv ++ arrInvVar aVarEnv aPtrEnv aEvalEnv).
 
 Definition kernelInv {GA} 
-           (aVarEnv : AVarEnv GA) (aPtrEnv : APtrEnv GA) (aEvalEnv : AEvalEnv GA) R P resEnv := 
-  Assn (arrInvRes aPtrEnv aEvalEnv *** R) P (resEnv ++ arrInvVar aVarEnv aPtrEnv aEvalEnv).
+           (aVarEnv : AVarEnv GA) (aPtrEnv : APtrEnv GA) (aEvalEnv : AEvalEnv GA) R P resEnv p := 
+  Assn (arrInvRes aPtrEnv aEvalEnv p *** R) P (resEnv ++ arrInvVar aVarEnv aPtrEnv aEvalEnv).
 
 Definition aenv_ok {GA} (avar_env : AVarEnv GA) :=
   (forall ty (m : member ty GA), prefix "l" (str_of_var (fst (hget avar_env m))) = false)
@@ -85,17 +85,17 @@ Definition func_ok1 {GA dom cod} (avar_env : AVarEnv GA)
      (* func only returs to local variables or parameter *)
      (forall x l, In l (flatTup (snd (func x))) -> is_local l) /\
      (* functional correctenss *)
-     (forall ntrd (tid : Fin.t ntrd) BS xs vs res aptr_env aeval_env R P resEnv,
+     (forall ntrd (tid : Fin.t ntrd) BS xs vs res aptr_env aeval_env R P resEnv p,
          (forall l, In l (flatTup xs) -> ~is_local l)
          -> (forall l v, In (l |-> v) resEnv -> ~is_local l)
          -> (Skel.funcDenote _ _ f aeval_env vs = Some res)
          -> CSL BS tid
-                (kernelInv avar_env aptr_env aeval_env R P 
-                           (xs |=> sc2CUDA vs ++ resEnv))
+                (kernelInv avar_env aptr_env aeval_env R P
+                           (xs |=> sc2CUDA vs ++ resEnv) p)
                 (fst (func xs))
                 (kernelInv avar_env aptr_env aeval_env R P
                            (snd (func xs) |=> sc2CUDA res ++
-                            xs |=> sc2CUDA vs ++ resEnv))) /\
+                            xs |=> sc2CUDA vs ++ resEnv) p)) /\
      (forall x, barriers (fst (func x)) = nil).
 
 Definition func_ok2 {GA dom1 dom2 cod} (avar_env : AVarEnv GA) 
@@ -106,18 +106,18 @@ Definition func_ok2 {GA dom1 dom2 cod} (avar_env : AVarEnv GA)
      (* func only returs to local variables or parameter *)
      (forall x y l, In l (flatTup (snd (func x y))) -> is_local l) /\
      (* functional correctenss *)
-     (forall ntrd (tid : Fin.t ntrd) BS xs ys vs1 vs2 res aptr_env aeval_env R P resEnv,
+     (forall ntrd (tid : Fin.t ntrd) BS xs ys vs1 vs2 res aptr_env aeval_env R P resEnv p,
          (forall l, In l (flatTup xs) -> ~is_local l)
          -> (forall l, In l (flatTup ys) -> ~is_local l)
          -> (forall l v, In (l |-> v) resEnv -> ~is_local l)
          -> (Skel.funcDenote _ _ f aeval_env vs1 vs2 = Some res)
          -> CSL BS tid
-                (kernelInv avar_env aptr_env aeval_env R P 
-                           (xs |=> sc2CUDA vs1 ++ ys |=> sc2CUDA vs2 ++ resEnv))
+                (kernelInv avar_env aptr_env aeval_env R P
+                           (xs |=> sc2CUDA vs1 ++ ys |=> sc2CUDA vs2 ++ resEnv) p)
                 (fst (func xs ys))
                 (kernelInv avar_env aptr_env aeval_env R P
                            (snd (func xs ys) |=> sc2CUDA res ++ 
-                            xs |=> sc2CUDA vs1 ++ ys |=> sc2CUDA vs2 ++ resEnv))) /\
+                            xs |=> sc2CUDA vs1 ++ ys |=> sc2CUDA vs2 ++ resEnv) p)) /\
      (forall xs ys, barriers (fst (func xs ys)) = nil).
 
 Definition func_ok {GA fty} (avar_env : AVarEnv GA) :=
@@ -143,15 +143,15 @@ Definition ae_ok {GA ty} (avar_env : AVarEnv GA) (ae : Skel.AE GA ty) (arr : var
      (* func only returs to local variables or parameter *)
      (forall x l, In l (flatTup (snd (arr x))) -> is_local l) /\
      (* functional correctenss *)
-     (forall ntrd (tid : Fin.t ntrd) BS ix i res aptr_env aeval_env R P resEnv,
+     (forall ntrd (tid : Fin.t ntrd) BS ix i res aptr_env aeval_env R P resEnv p,
          ~is_local ix
          -> (forall l v, In (l |-> v) resEnv -> ~is_local l)
          -> (Skel.aeDenote _ _ ae aeval_env = Some res)
          -> i < length res
          -> CSL BS tid
                 (kernelInv avar_env aptr_env aeval_env R P 
-                           (ix |-> Zn i :: resEnv))
+                           (ix |-> Zn i :: resEnv) p)
                 (fst (arr ix))
                 (kernelInv avar_env aptr_env aeval_env R P
-                           ((snd (arr ix)) |=> sc2CUDA (gets' res i) ++ ix |-> Zn i :: resEnv))) /\
+                           ((snd (arr ix)) |=> sc2CUDA (gets' res i) ++ ix |-> Zn i :: resEnv) p)) /\
      (forall x, barriers (fst (arr x)) = nil).
